binary op equality typing lemmas

deps/poulet4/lib/LightTyping/Utility.v
@@ -3,8 +3,6 @@ Require Export Coq.micromega.Lia Poulet4.ValueUtil
 Require Import Poulet4.Monads.Monad Poulet4.Monads.Option
         VST.zlist.sublist Poulet4.Utils.
 
-Notation predopt := (EquivUtil.predop).
-
 Section Utils.
   Context {tags_t : Type}.
   Notation typ  := (@P4Type tags_t).
@@ -42,6 +40,39 @@ Section Utils.
   Proof.
     intros ? ? ? H; inversion H; subst; auto.
   Qed.
+
+  (** Types of terms that may be compared for equality. *)
+  Inductive Eq_type : typ -> Prop :=
+  | Eq_Error :
+      Eq_type TypError
+  | Eq_Enum E t mems :
+      predop Eq_type t ->
+      Eq_type (TypEnum E t mems)
+  | Eq_Bool :
+      Eq_type TypBool
+  | Eq_Bit w :
+      Eq_type (TypBit w)
+  | Eq_Int w :
+      Eq_type (TypInt w)
+  | Eq_VarBit w :
+      Eq_type (TypVarBit w)
+  | Eq_Integer :
+      Eq_type TypInteger
+  | Eq_Struct xts :
+      Forall (Eq_type ∘ snd) xts ->
+      Eq_type (TypStruct xts)
+  | Eq_Union xts :
+      Forall (Eq_type ∘ snd) xts ->
+      Eq_type (TypHeaderUnion xts)
+  | Eq_Header xts :
+      Forall (Eq_type ∘ snd) xts ->
+      Eq_type (TypHeaderUnion xts)
+  | Eq_Tuple ts :
+      Forall Eq_type ts ->
+      Eq_type (TypTuple ts)
+  | Eq_Array t n :
+      Eq_type t ->
+      Eq_type (TypArray t n).
   
   (** Evidence a binary operation is valid for given types. *)
   Variant binary_type : OpBin -> typ -> typ -> typ -> Prop :=
@@ -64,8 +95,10 @@ Section Utils.
       numeric t1 ->
       binary_type Shr t1 TypInteger t1
   | BTEq t :
+      Eq_type t ->
       binary_type Eq t t TypBool
   | BTNotEq t :
+      Eq_type t ->
       binary_type NotEq t t TypBool
   | BTPlus t :
       numeric t ->
@@ -248,10 +281,151 @@ Ltac inv_numeric :=
   | H: numeric _ |- _ => inversion H; subst; try inv_numeric_width
   end.
 
+Section EqTypeInd.
+  Variable tags_t : Type.
+  Notation typ := (@P4Type tags_t).
+  Variable P : typ -> Prop.
+
+  Hypothesis HError : P TypError.
+  Hypothesis HEnum : forall E t mems,
+      predop Eq_type t ->
+      predop P t ->
+      P (TypEnum E t mems).
+  Hypothesis HBool : P TypBool.
+  Hypothesis HBit : forall w, P (TypBit w).
+  Hypothesis HInt : forall w, P (TypInt w).
+  Hypothesis HVarBit : forall w, P (TypVarBit w).
+  Hypothesis HInteger : P TypInteger.
+  Hypothesis HStruct : forall xts,
+      Forall (Eq_type ∘ snd) xts ->
+      Forall (P ∘ snd) xts ->
+      P (TypStruct xts).
+  Hypothesis HUnion : forall xts,
+      Forall (Eq_type ∘ snd) xts ->
+      Forall (P ∘ snd) xts ->
+      P (TypHeaderUnion xts).
+  Hypothesis HHeader : forall xts,
+      Forall (Eq_type ∘ snd) xts ->
+      Forall (P ∘ snd) xts ->
+      P (TypHeaderUnion xts).
+  Hypothesis HTuple : forall ts,
+      Forall Eq_type ts ->
+      Forall P ts ->
+      P (TypTuple ts).
+  Hypothesis HArray : forall t n,
+      Eq_type t ->
+      P t ->
+      P (TypArray t n).
+
+  Definition my_Eq_type_ind :
+    forall t : typ, Eq_type t -> P t :=
+    fix I t H :=
+      let PI {t} (H: predop Eq_type t) : predop P t :=
+          match H with
+          | predop_none _     => predop_none _
+          | predop_some _ _ H => predop_some _ _ (I _ H)
+          end in
+      let fix LI {ts} (H: Forall Eq_type ts) : Forall P ts :=
+          match H with
+          | Forall_nil _        => Forall_nil _
+          | Forall_cons _ Hh Ht => Forall_cons _ (I _ Hh) (LI Ht)
+          end in
+      let fix ALI {xts} (H: Forall (Eq_type ∘ snd) xts)
+          : Forall (P ∘ snd) xts :=
+          match H with
+          | Forall_nil _        => Forall_nil _
+          | Forall_cons _ Hh Ht => Forall_cons _ (I _ Hh) (ALI Ht)
+          end in
+      match H with
+      | Eq_Error        => HError
+      | Eq_Enum E _ m H => HEnum E _ m H (PI H)
+      | Eq_Bool         => HBool
+      | Eq_Bit w        => HBit w
+      | Eq_Int w        => HInt w
+      | Eq_Integer      => HInteger
+      | Eq_VarBit w     => HVarBit w
+      | Eq_Array _ n H  => HArray _ n H (I _ H)
+      | Eq_Struct _ H   => HStruct _ H (ALI H)
+      | Eq_Header _ H   => HHeader _ H (ALI H)
+      | Eq_Union  _ H   => HUnion  _ H (ALI H)
+      | Eq_Tuple  _ H   => HTuple  _ H (LI H)
+      end.
+End EqTypeInd.
+
+Ltac some_inv :=
+  match goal with
+  | H: Some _ = Some _ |- _ => inversion H; subst; clear H
+  end.
+
+Ltac match_some_inv :=
+  match goal with
+  | H: match ?trm with Some _ => _ | None => _ end = Some _
+    |- _ => destruct trm as [? |] eqn:? ; cbn in *;
+          try discriminate
+  end.
+
+Ltac if_destruct :=
+  match goal with
+  | H: context [if ?t then _ else _] |- _
+    => destruct t eqn:?; cbn in *; try discriminate; try some_inv
+  | |- context [if ?t then _ else _]
+    => destruct t eqn:?; cbn in *; try discriminate; try some_inv
+  end.
+
 Section Lemmas.
   Context {tags_t : Type}.
   Notation typ := (@P4Type tags_t).
+
+  Local Hint Constructors binary_type : core.
+  Local Hint Constructors numeric_width : core.
+  Local Hint Constructors numeric : core.
+  Local Hint Constructors Eq_type : core.
+  Local Hint Constructors predop : core.
+
+  Ltac rw_Forall_map H :=
+    pose proof Forall_map (@Eq_type tags_t) normᵗ as H';
+    unfold "∘" in H'; rewrite <- H' in H; clear H'.
   
+  Lemma Eq_type_normᵗ : forall t : typ,
+      Eq_type t -> Eq_type (normᵗ t).
+  Proof.
+    intros t H; induction H using my_Eq_type_ind;
+      cbn in *; auto;
+        try match goal with
+            | H: Forall ((fun t : typ => Eq_type (normᵗ t)) ∘ snd) ?xts
+              |- context [map (fun '(x, t) => (x, normᵗ t)) ?xts]
+              => constructor;
+                  rewrite <- Forall_map with (g:=snd) in *;
+                  rewrite map_snd_map; rw_Forall_map H; assumption
+            end.
+    - inversion H0; subst; cbn in *; auto.
+    - rw_Forall_map H0; auto.
+  Qed.
+
+  Local Hint Resolve Eq_type_normᵗ : core.
+
+  Lemma numeric_width_normᵗ : forall w (t : typ),
+      numeric_width w t -> numeric_width w (normᵗ t).
+  Proof.
+    intros w t H; inv_numeric_width; auto.
+  Qed.
+
+  Local Hint Resolve numeric_width_normᵗ : core.
+  
+  Lemma numeric_normᵗ : forall t : typ,
+      numeric t -> numeric (normᵗ t).
+  Proof.
+    intros t H; inv_numeric; auto.
+  Qed.
+
+  Local Hint Resolve numeric_normᵗ : core.
+  
+  Lemma binary_type_normᵗ : forall o (r r1 r2 : typ),
+      binary_type o r1 r2 r -> binary_type o (normᵗ r1) (normᵗ r2) (normᵗ r).
+  Proof.
+    intros o r r1 r2 Hbt; inversion Hbt; subst; cbn; eauto.
+  Qed.
+
   Lemma is_expr_typ_list_uninit_sval_of_typ :
     forall (ts : list (typ)) b,
       Forall is_expr_typ ts ->
@@ -322,7 +496,7 @@ Section Lemmas.
     rewrite Hmap; clear Hmap.
     unfold ">>|", ">>=".
     unfold option_monad_inst,
-    option_bind, option_ret, mret in *.
+    option_bind, mret in *.
     repeat rewrite Utils.map_pat_both.
     clear Hok Hxts IHxts.
     generalize dependent vs.
@@ -364,46 +538,45 @@ Section Lemmas.
         | t n Ht IHt (* array *)
         | ts Hts IHts (* tuple *)
         | ts Hts IHts (* list *)
-        | xts Hxts IHxts (* record *)
+        | xts Uxts Hxts IHxts (* record *)
         | (* error *)
-        | xts Hxts IHxts (* header *)
-        | xts Hxts IHxts (* union *)
-        | xts Hxts IHxts (* struct *)
+        | xts Uxts Hxts IHxts (* header *)
+        | xts Uxts Hxts IHxts (* union *)
+        | xts Uxts Hxts IHxts (* struct *)
         | X ms Hms       (* enum *)
         | X t ms Ht IHt (* senum *)
         | X (* name *)
         | X t Ht IHt (* newtype *)
         ] using my_is_expr_typ_ind;
       inversion Hok; subst; cbn in *;
-        unfold option_monad_inst,
-        option_bind, option_ret in *;
+        unfold option_monad_inst, option_bind in *;
         try contradiction; eauto.
     - assert (H0n: (0 <? n)%N = true) by (rewrite N.ltb_lt; lia).
       rewrite H0n; eauto.
     - eapply is_expr_typ_list_uninit_sval_of_typ
         in Hts as [vs Hvs]; eauto.
       unfold option_monad_inst,
-      option_bind, option_ret in Hvs; rewrite Hvs; eauto.
+      option_bind in Hvs; rewrite Hvs; eauto.
     - eapply is_expr_typ_list_uninit_sval_of_typ
         in Hts as [vs Hvs]; eauto.
       unfold option_monad_inst,
-      option_bind, option_ret in Hvs; rewrite Hvs; eauto.
+      option_bind in Hvs; rewrite Hvs; eauto.
     - eapply is_expr_typ_alist_uninit_sval_of_typ
         in Hxts as [xvs Hxvs]; eauto.
       unfold ">>|",">>=",mret, option_monad_inst,
-      option_bind, option_ret in Hxvs; rewrite Hxvs; eauto.
+      option_bind in Hxvs; rewrite Hxvs; eauto.
     - eapply is_expr_typ_alist_uninit_sval_of_typ
         in Hxts as [xvs Hxvs]; eauto.
       unfold ">>|",">>=",mret, option_monad_inst,
-      option_bind, option_ret in Hxvs; rewrite Hxvs; eauto.
+      option_bind in Hxvs; rewrite Hxvs; eauto.
     - eapply is_expr_typ_alist_uninit_sval_of_typ
         in Hxts as [xvs Hxvs]; eauto.
       unfold ">>|",">>=",mret, option_monad_inst, 
-      option_bind, option_ret in Hxvs; rewrite Hxvs; eauto.
+      option_bind in Hxvs; rewrite Hxvs; eauto.
     - eapply is_expr_typ_alist_uninit_sval_of_typ
         in Hxts as [xvs Hxvs]; eauto.
       unfold ">>|",">>=",mret, option_monad_inst, 
-      option_bind, option_ret in Hxvs; rewrite Hxvs; eauto.
+      option_bind in Hxvs; rewrite Hxvs; eauto.
     - destruct X as [d X];
         destruct ms as [| [i M] ms];
         simpl in *; try lia; eauto.
@@ -492,15 +665,21 @@ Section Lemmas.
   Local Hint Extern 0 => bruh_list : core.
   
   Ltac bruh_alist :=
-    intros xts' IHxts' Hxts';
-    injection Hxts' as ?; subst;
-    constructor;
-    rewrite Forall_forall in *;
-    intros [x t] Hxt; cbn in *;
     match goal with
-    | H: List.In _ ?l,
-         IH: context [List.In _ (map ?g ?l)]
-      |- _ => apply in_map with (f := g) in H as Hinmap; eauto
+    | Uxts: AList.key_unique _ = true
+      |- _ => intros xts' IHxts' Hxts';
+            injection Hxts' as ?; subst;
+            epose proof AList.key_unique_map_values as Hmv;
+            unfold AList.map_values in Hmv;
+            rewrite Hmv in Uxts; clear Hmv;
+            constructor; auto;
+            rewrite Forall_forall in *;
+            intros [x t] Hxt; cbn in *;
+            match goal with
+            | H: List.In _ ?l,
+                 IH: context [List.In _ (map ?g ?l)]
+              |- _ => apply in_map with (f := g) in H as Hinmap; eauto
+            end
     end.
 
   Local Hint Extern 0 => bruh_alist : core.
@@ -521,11 +700,11 @@ Section Lemmas.
         | t n Ht IHt (* array *)
         | ts Hts IHts (* tuple *)
         | ts Hts IHts (* list *)
-        | xts Hxts IHxts (* record *)
+        | xts Uxts Hxts IHxts (* record *)
         | (* error *)
-        | xts Hxts IHxts (* header *)
-        | xts Hxts IHxts (* union *)
-        | xts Hxts IHxts (* struct *)
+        | xts Uxts Hxts IHxts (* header *)
+        | xts Uxts Hxts IHxts (* union *)
+        | xts Uxts Hxts IHxts (* struct *)
         | X ms Hms       (* enum *)
         | X t ms Ht IHt (* senum *)
         | X (* name *)
@@ -576,7 +755,7 @@ Section Lemmas.
     rewrite <- map_map with
         (g := normᵗ) (f := snd) in Hxts;
     rewrite map_pat_combine, map_id;
-    unfold option_ret, option_bind;
+    unfold option_bind;
     induction xts as [| [[i x] t] xts IHxts];
     simpl in *; inversion Hxts; subst; f_equal; auto; assumption.
   
